[Dafny] Clean up + Comment dafny_compilerProgScript

compiler/dafny_new/translation/dafny_compilerProgScript.sml
@@ -19,24 +19,33 @@ val _ = new_theory "dafny_compilerProg";
 
 val _ = translation_extends "dafny_transformProg";
 
+(* First, we translate the functions for converting the output of the compiler
+   (CakeML AST) into an S-expression string, namely decsexp, listsexp, and
+   print_sexp *)
+
+(* Adapted from compiler/bootstrap/translation/sexp_parserProgScript.sml *)
+
+(* Note that we keep turning on and off use_string_type. This appears to be
+   necessary to avoid weird translation problems, especially starting with the
+   translation of litsexp_def for some reason, which is also where the on/offs
+   start to differ from sexp_parserProg. The downside is, that this seems to
+   introduce *a lot* of automatic additions of IMPLODE sometimes; see TODOs. *)
+
 val _ = ml_translatorLib.use_string_type true;
 val _ = ml_translatorLib.use_sub_check true;
-
-val r = translate stringTheory.isPrint_def
-val _ = ml_translatorLib.use_string_type false;
-
 val _ = add_preferred_thy "-";
 
-val _ = ml_translatorLib.use_string_type true;
+val r = translate stringTheory.isPrint_def;
 
 Theorem strip_dot_alt =
   simpleSexpParseTheory.strip_dot_def |> PURE_ONCE_REWRITE_RULE [CONS_APPEND];
-val _ = translate strip_dot_alt
 
-val _ = translate simpleSexpParseTheory.print_space_separated_def;
+val r = translate strip_dot_alt;
+
+val r = translate simpleSexpParseTheory.print_space_separated_def;
 
 val _ = use_string_type false;
-val _ = translate simpleSexpParseTheory.escape_string_def;
+val r = translate simpleSexpParseTheory.escape_string_def;
 val _ = use_string_type true;
 
 Theorem num_to_dec_string_v_thm:
@@ -49,6 +58,7 @@ QED
 
 val _ = add_user_proved_v_thm num_to_dec_string_v_thm;
 
+(* The following TODO was copied over from sexp_parserProgScript.sml *)
 (* TODO: translator failed for some reason if I just prove these as equations on print_sexp *)
 Definition print_sexp_alt_def:
   (print_sexp_alt (SX_SYM s) = s) ∧
@@ -64,7 +74,7 @@ Definition print_sexp_alt_def:
    | SOME lst =>
        "(" ++ print_space_separated (MAP print_sexp_alt ls) ++ " . " ++ print_sexp_alt lst ++ ")")
 Termination
-  WF_REL_TAC`measure sexp_size` >> rw[] >> simp[simpleSexpTheory.sexp_size_def] >>
+  WF_REL_TAC‘measure sexp_size’ >> rw[] >> simp[simpleSexpTheory.sexp_size_def] >>
    fs[Once simpleSexpParseTheory.strip_dot_def] >>
    pairarg_tac \\ fs[] \\ rw[simpleSexpTheory.sexp_size_def] \\ fs[]
    \\ imp_res_tac simpleSexpParseTheory.strip_dot_MEM_sizelt
@@ -83,11 +93,11 @@ QED
 Theorem print_sexp_alt_thm:
   print_sexp s = print_sexp_alt s
 Proof
-  `?n. n = sexp_size s` by rw[] >>
+  ‘∃n. n = sexp_size s’ by rw[] >>
   pop_assum mp_tac >>
-  qid_spec_tac `s` >> qid_spec_tac `n` >>
+  qid_spec_tac ‘s’ >> qid_spec_tac ‘n’ >>
   ho_match_mp_tac COMPLETE_INDUCTION >>
-  rpt strip_tac >> Cases_on `s` >>
+  rpt strip_tac >> Cases_on ‘s’ >>
   fs[simpleSexpParseTheory.print_sexp_def,print_sexp_alt_def,IMPLODE_EXPLODE_I,
      sexp_size_def, PULL_FORALL] >>
   pairarg_tac >> fs[] >> every_case_tac >>
@@ -113,23 +123,20 @@ QED
 
 val r = translate EL;
 
-val el_side = Q.prove(
-  `!n xs. el_side n xs = (n < LENGTH xs)`,
-  Induct THEN Cases_on `xs` THEN ONCE_REWRITE_TAC [fetch "-" "el_side_def"]
-  THEN fs[])
-                |> update_precondition;
+Triviality el_side_thm:
+  ∀n xs. el_side n xs = (n < LENGTH xs)
+Proof
+  Induct THEN Cases_on ‘xs’ THEN ONCE_REWRITE_TAC [fetch "-" "el_side_def"]
+  THEN fs[]
+QED
 
-val _ = translate print_sexp_alt_def;
+val _ = el_side_thm |> update_precondition;
 
-val _ = translate print_sexp_alt_thm;
+val r = translate print_sexp_alt_def;
 
-
-(* CUT *)
+val r = translate print_sexp_alt_thm;
 
 val _ = use_string_type false;
-val _ = use_sub_check false;
-
-(* --- *)
 
 Triviality listsexp_alt:
   listsexp = FOLDR (λs1 s2. SX_CONS s1 s2) nil
@@ -137,33 +144,34 @@ Proof
   rpt(CHANGED_TAC(CONV_TAC (DEPTH_CONV ETA_CONV))) >> simp[listsexp_def]
 QED
 
-val _ = translate listsexp_alt;
+val r = translate listsexp_alt;
 
-(* --- *)
+val r = translate (fromSexpTheory.locnsexp_def |> SIMP_RULE list_ss []);
+val r = translate fromSexpTheory.locssexp_def;
 
-val _ = translate (fromSexpTheory.locnsexp_def |> SIMP_RULE list_ss []);  (* TODO is this necessary *)
-val _ = translate fromSexpTheory.locssexp_def;
-
-(* --- *)
-
-val _ = translate HEX_def
+val r = translate ASCIInumbersTheory.HEX_def;
 
 Definition hex_alt_def:
   hex_alt x = if x < 16 then HEX x else #"0"
 End
 
-val _ = translate hex_alt_def
+val r = translate hex_alt_def;
 
-val _ = Q.prove(`!n. hex_alt_side n <=> T`,
- PURE_REWRITE_TAC[fetch "-" "hex_alt_side_def",fetch "-" "hex_side_def"] >>
- intLib.COOPER_TAC) |> update_precondition;
+Triviality hex_alt_side_thm:
+  ∀n. hex_alt_side n ⇔ T
+Proof
+  PURE_REWRITE_TAC [fetch "-" "hex_alt_side_def",fetch "-" "hex_side_def"]
+  >> intLib.COOPER_TAC
+QED
+
+val _ = hex_alt_side_thm |> update_precondition;
 
 Definition num_to_hex_string_alt:
   num_to_hex_string_alt = n2s 16 hex_alt
 End
 
 Theorem num_to_hex_string_alt_intro:
-  !n. num_to_hex_string n = num_to_hex_string_alt n
+  ∀n. num_to_hex_string n = num_to_hex_string_alt n
 Proof
   simp[num_to_hex_string_def,num_to_hex_string_alt,n2s_def] >>
   ho_match_mp_tac COMPLETE_INDUCTION >>
@@ -172,52 +180,71 @@ Proof
   rw[hex_alt_def]
 QED
 
-val _ = translate numposrepTheory.n2l_def;
+val r = translate numposrepTheory.n2l_def;
 
-val n2l_side_thm = Q.prove(`!n m. n2l_side n m <=> n <> 0`,
+Triviality n2l_side_thm:
+  ∀n m. n2l_side n m ⇔ n ≠ 0
+Proof
   strip_tac >>
   ho_match_mp_tac COMPLETE_INDUCTION >>
   rpt strip_tac >>
   PURE_ONCE_REWRITE_TAC[fetch "-" "n2l_side_def"] >>
-  rw[]) |> update_precondition
+  rw[]
+QED
 
-val  _ = translate n2s_def;
+val _ = n2l_side_thm |> update_precondition;
 
-val n2s_side_thm = Q.prove(`!n f m. n2s_side n f m <=> n <> 0`,
+
+val r = translate ASCIInumbersTheory.n2s_def;
+
+Triviality n2s_side_thm:
+  ∀n f m. n2s_side n f m ⇔ n ≠ 0
+Proof
   rpt strip_tac >>
   PURE_ONCE_REWRITE_TAC[fetch "-" "n2s_side_def"] >>
-  rw[n2l_side_thm]) |> update_precondition
+  rw[n2l_side_thm]
+QED
 
-val _ = translate num_to_hex_string_alt;
+val _ = n2s_side_thm |> update_precondition;
 
-val _ = translate num_to_hex_string_alt_intro;
 
-(* --- *)
+val r = translate num_to_hex_string_alt;
+
+val r = translate num_to_hex_string_alt_intro;
+
 
 val r = translate fromSexpTheory.encode_control_def;
 
-val _ = translate fromSexpTheory.SEXSTR_def;
+val r = translate fromSexpTheory.SEXSTR_def;
 
 val _ = ml_translatorLib.use_string_type false;
-val _ = translate fromSexpTheory.litsexp_def;
-val litsexp_side_thm = Q.prove(`!v. litsexp_side v <=> T`,
-  PURE_ONCE_REWRITE_TAC[fetch "-" "litsexp_side_def"] >> rw[] >>
-                               intLib.COOPER_TAC) |> update_precondition
 
-val _ = translate optsexp_def;
-val _ = translate idsexp_def;
-val _ = translate typesexp_def;
+val r = translate fromSexpTheory.litsexp_def;
 
-val _ = translate fromSexpTheory.patsexp_def;
+Triviality litsexp_side_thm:
+  ∀v. litsexp_side v ⇔ T
+Proof
+  PURE_ONCE_REWRITE_TAC[fetch "-" "litsexp_side_def"] >> rw[]
+  >> intLib.COOPER_TAC
+QED
 
-val _ = translate opsexp_def;
-val _ = translate lopsexp_def;
-val _ = translate scsexp_def;
-val _ = translate expsexp_def;
+val _ = litsexp_side_thm |> update_precondition;
 
-val _ = translate type_defsexp_def;
+val r = translate fromSexpTheory.optsexp_def;
+val r = translate fromSexpTheory.idsexp_def;
+val r = translate fromSexpTheory.typesexp_def;
+val r = translate fromSexpTheory.patsexp_def;
+(* TODO 101 automatically added string IMPLODEs *)
+val r = translate fromSexpTheory.opsexp_def;
+val r = translate fromSexpTheory.lopsexp_def;
+val r = translate fromSexpTheory.scsexp_def;
+(* TODO 24 automatically added string IMPLODEs *)
+val r = translate fromSexpTheory.expsexp_def;
+val r = translate fromSexpTheory.type_defsexp_def;
+(* TODO 14 automatically added string IMPLODEs *)
+val r = translate fromSexpTheory.decsexp_def;
 
-val _ = translate fromSexpTheory.decsexp_def;
+(* Translating dafny_compilerTheory *)
 
 val r = translate dafny_compilerTheory.dfy_to_cml_def;
 val r = translate dafny_compilerTheory.unpack_def;
@@ -226,6 +253,8 @@ val r = translate dafny_compilerTheory.cmlm_to_str_def;
 val _ = ml_translatorLib.use_string_type true;
 
 val r = translate dafny_compilerTheory.main_function_def;
+
+(* Sanity checks + Finalizing *)
 
 val _ = type_of “main_function” = “:mlstring -> mlstring”
         orelse failwith "The main_function has the wrong type.";
